- if $\alpha^2<\omega_0^2$
- let $\omega'^{2} =\omega_{0}^{2}-\alpha^{2}$
- general solution: $$x(t)= e^{-\alpha t}(Ce^{i\omega'^{2}t}+De^{-i\omega'^{2}t})$$
- similar to underdamped case, *but* $e^{-\alpha t}$ implies an exponential decay to the amplitude and a modified "resonance" frequency: $$\omega'=\sqrt{\omega_{0}^{2}-\alpha^{2}}=\sqrt{\frac{k}{m}- \frac{\gamma^{2}}{4m^{2}}}$$
- for the initial conditions: $x(0)=x_{0,}\;v(0)=0$
		$x(0)=C+D=x_0$
		$(i \omega'-\alpha)C - (i\omega'D + \alpha)=0 \implies D= \frac{i\omega'-\alpha}{2i\omega'}x_{0} \, , \, C= \frac{i\omega'+\alpha}{2i\omega'}x_{0}$ 
		$$x(t) = \frac{x_{0}}{2\omega'}e^{-\alpha t} \left( (\omega'+ \frac{\alpha}{i})e^{\omega't} + (\omega'- \frac{\alpha}{i})e^{-\omega't} \right)$$
		$$\therefore x(t) = x_{0}e^{-\alpha t} \left( \cos{\omega't}+ \frac{\alpha}{\omega'}\sin\alpha t \right)$$ 