- $\alpha^2=\omega_0^2$
- guess solution: $x(t)=Ae^{\lambda t}$
		$\lambda^{2}+ 2\alpha \lambda + \omega_{0}^{2}=0$
		$\lambda_{1}=-\alpha+\sqrt{\alpha^{2}-\omega_{0}^{2}} \, , \, \lambda_{2}=-\alpha+\sqrt{\alpha^{2}-\omega_{0}^{2}}$
- only one solution: $\lambda = -\alpha$
- **must** have two constants of integration for the second order differential equation, therefore there must be another term
- postulate a second solution: $$x(t)=Dte^{\lambda t}=Dte^{-\alpha t}$$ $$\frac{dx}{dt}= De^{-\alpha t}(1-\alpha t)$$ $$\frac{d^{2}x}{dt^{2}}= \alpha De^{-\alpha t}(\alpha t-2)$$
- substitute these into the equation of motion [[PX153 - B5 - application - describing damped smh#^efbd92|here]]: $$\alpha(\alpha t -2)De^{\alpha t} + 2 \alpha(1-\alpha t) De^{-\alpha t} + \omega_{0}^{2}tDe^{-\alpha t} =0$$
- for these to be true at all times: $$\alpha^{2}t-2\alpha+2\alpha-2\alpha^{2}t+\omega_{0}^{2}t=0$$ $$(\omega_0^2-\alpha^2)t=0$$
- for the initial conditions $x(0)=x_{0}$ , $v(0)=0$:
		$x_{0}=C$
		$-\alpha C + D = 0$
$$\therefore x(t) = x_0(e^{-\alpha t} + \alpha t e^{-\alpha t})$$
