- $\alpha^2>\omega_0^2$
- let $\kappa=\sqrt{\alpha^2-\omega_0}$
- general solution:$$x(t)= e^{-\alpha t}(Ce^{\kappa t}+De^{-\kappa t})$$
- there is no oscillation
- for the initial conditions: $x(0)=x_{0,}\;v(0)=0$
		$x(0)=C+D=x_0$
		$(\kappa-\alpha)C - (\kappa + \alpha)D=0 \implies D= \frac{\kappa-\alpha}{2\kappa}x_{0} \, , \, C= \frac{\kappa+\alpha}{2\kappa}x_{0}$ 
		$$\therefore x(t) = \frac{x_{0}}{2\kappa}e^{-\alpha t} \left( (\kappa + \alpha)e^{\kappa t} + (\kappa-\alpha)e^{-\kappa t} \right)$$ 
- for long times: $e^{\kappa t}>> e^{-\kappa t}$ $\implies x(t)\to e^{-\alpha t}\cdot e^{\kappa t}=e^{-(\alpha - \kappa)t}$
	- ie: exponential decay with time constant longer than $\frac{1}{\alpha}$
