- a fundamental equation, ubiquitous in physics
- the wave function: $$u(x,t) = A\cos(kx-\omega t)$$
- differentiating wrt $t$: $$\frac{\partial u}{\partial t} = A\omega\sin(kx-\omega t)$$
	- **note**: $\frac{\partial u}{\partial t} \neq v$
- for acceleration: $$\begin{align*}
	\frac{\partial^{2} u}{\partial t^{2}} &= -A\omega^{2}\cos(kx-\omega t) \\
	\frac{\partial^{2} u}{\partial t^{2}} &= -\omega^{2} \, u(x,t) \; ...[1]
\end{align*}$$
- differentiating wrt ${} x$: $$\frac{\partial u}{\partial x} = -Ak\sin(kx-\omega t)$$
- again: $$\begin{align*}
	\frac{\partial^{2} u}{\partial x^{2}} = -Ak^{2}\sin(kx-\omega t) \\
	\frac{\partial^{2} u}{\partial x^{2}} = -k^{2} \, u(x,t)  \; ...[2]
\end{align*}$$
- from $[1]$ and $[2]$: $$\begin{align*}
	\frac{1}{k^{2}} \frac{\partial^{2} u}{\partial x^{2}} &= \frac{1}{\omega^{2}}\frac{\partial^{2} u}{\partial t^{2}} \\
	\frac{\partial^{2} u}{\partial t^{2}} &= \frac{\omega^{2}}{k^{2}}\frac{\partial^{2} u}{\partial x^{2}}
\end{align*}$$
- the wave equation: $$\frac{\partial^{2} u}{\partial t^{2}} = v^{2} \, \frac{\partial^{2} u}{\partial x^{2}}$$ [YF eqn 15.12] ^c8f14b
- ***comments***:
	- applies to right + left travelling waves, and also to standing waves
	- this is in 1D, in 3D: $$\frac{\partial^{2} u}{\partial t^{2}} =  v^{2} \, \vec \nabla^{2} u$$
			where: $\vec\nabla^{2}u = (\frac{\partial^{2}}{\partial x^{2}} + \frac{\partial^{2}}{\partial y^{2}} + \frac{\partial^{2}}{\partial z^{2}})u$
- electromagnetic waves: $$\frac{\partial^{2} E}{\partial t^{2}} = \frac{1}{\mu_{0}\epsilon_{0}} \, \frac{\partial^{2} E}{\partial x^{2}}$$
		where, $E=$ electric field, $\mu_{0}=$ permeability of free space, $\epsilon_0=$ permittivity of free space
	- we can see here: $$c = \frac{1}{\sqrt{\mu_{0}\epsilon_{0}}} = 3\times 10^{8}ms^{-1}$$
	