## capacitance
![[Pasted image 20240131101020.png]]
$$C = \frac{Q}{V}$$
- units: $C\,V^{-1}$ or $farad\,(F)$
## parallel plate capacitor
- electric field: $$\vec E = \vec E_{top} + \vec E_{bottom} = - \frac{\sigma}{\epsilon_{0}}\hat{z}$$
		where, $\sigma= \frac{Q}{A}$ : surface charge density
- potential difference between the plates: $$V = E\, d = \frac{\sigma}{\epsilon_{0}}d = \frac{Qd}{\epsilon_{0}A}$$
- for parallel plates: $$C = \frac{Q}{V} = \frac{\epsilon_{0}A}{d}$$
## cylindrical capacitor
![[Pasted image 20240131101036.png]]
$$\begin{align*}
	V_{ab} &= \frac{\lambda}{2\pi\epsilon_{0}} \ln\left(\frac{R_{b}}{R_{a}}\right) \\
	&= \frac{Q}{2\pi\epsilon_{0}L} \ln\left(\frac{R_{b}}{R_{a}}\right) \\
\end{align*}$$
$$\therefore C = \frac{2\pi\epsilon_{0}L}{\ln(\frac{R_{b}}{R_{a}})}$$
## spherical capacitor
![[Pasted image 20240131101054.png]]
$$q = \sigma_{a}4\pi r_{a}^{2} = -\sigma_{b}4\pi r_{b}^{2}$$
$$V_{ab} = \frac{q}{4\pi\epsilon_{0}} \left(\frac{1}{r_{a}}- \frac{1}{r_{b}}\right)$$
$$C = \frac{4\pi\epsilon_{0}}{(\frac{1}{r_{a}}- \frac{1}{r_{b}})}$$
- single-plate spherical capacitor: **van der graaf generator**
## capacitors in series
![[Pasted image 20240131101121.png]]
- conservation of charge: both capacitors have the same charge, $Q:$ $$V_{1}= \frac{Q}{C_{1}}\;,\;V_{2}=\frac{Q}{C_{2}}$$
$$\implies V = V_{1} + V_{2} = Q \left(\frac{1}{C_{1}} + \frac{1}{C_{2}}\right)$$
- this is equivalent to a circuit with one capacitor, $C_{eq}$: $$\frac{1}{C_{eq}} = \frac{1}{C_{1}}+ \frac{1}{C_{2}}$$
- assume both the capacitors have the same $A$ and $\epsilon_{0}:$ $$\frac{1}{C_{eq}} = \frac{d_{1}}{\epsilon_{0}A} + \frac{d_{2}}{\epsilon_{0}A} = \frac{d_{1}+d_{2}}{\epsilon_{0}A} $$
## capacitors in parallel
![[Pasted image 20240131101149.png]] 
- both capacitors have the same potential drop
$$Q_{1} =C_{1}V \; ,\; Q_{2}=C_{2}V$$
- total charge: $Q = Q_{1}+Q_{2} = (C_{1}+C_{2})V$
- equivalent capacitor, $C_{eq}:$ $$C_{eq} = C_{1}+C_{2}$$

- eg: two capacitors have the same separation, $d$, and $\epsilon_0$
	$$C_{eq} = \frac{\epsilon_{0}A_{1}}{d} + \frac{\epsilon_{0}A_{2}}{d} = \frac{\epsilon_{0}}{d}(A_{1}+A_{2})$$