- total force, $\vec F_{0}$, on charge, $q_{0}$ : $$\vec F_{0} = \sum\limits_{i=1}^{N} \vec F_{i0} = \frac{q_{0}}{4\pi\epsilon_{0}} \sum\limits_{i=0}^{N} q_{i} \frac{\vec r_{0} - \vec r_{i}}{|\vec r_{0} - \vec r_{i}|^{3}}$$
- eg: ![[Pasted image 20240110093525.png]]
	$q_{1}=q_{2}=q$
	$\vec r_{1}= d \hat y$ and $\vec r_{2} = -d \hat y$
	$\vec r_{Q}= x \hat x$
	$$\begin{align}

    \vec F_{Q} &= \frac{Q q_{1}}{4\pi\epsilon_{0}} \frac{\vec r_{Q} - \vec r_{1}}{|\vec r_{Q} - \vec r_{1}|^{3}} + \frac{Q q_{2}}{4\pi\epsilon_{0}} \frac{\vec r_{Q} - \vec r_{2}}{|\vec r_{Q} - \vec r_{2}|^{3}} \\
    
	&= \frac{Q q_{1}}{4\pi\epsilon_{0}} \left\{ \frac{x\hat x -d\hat y}{(x^{2}+d^{2})^{\frac{3}{2}}} + \frac{x\hat x +d\hat y}{(x^{2}+d^{2})^{\frac{3}{2}}}\right\} \\
	
	\therefore \vec F_{Q} &= \frac{Q q_{1}}{4\pi\epsilon_{0}} \frac{2x\hat x}{(x^{2}+d^{2})^{\frac{3}{2}}} 
	\end{align}$$
 